Added all invariants to statement of uf_merge_invariant. Added cong_closure.v from Devi.

cong_closure.v
@@ -1,172 +1,754 @@
 Require Import Coq.Lists.List.
-
 Require Import Coq.Classes.EquivDec.
+Require Import Coq.Init.Nat.
+Require Import Coq.Arith.EqNat.
+Require Import Coq.Arith.PeanoNat.
 
+Require Import Coq.Program.Wf.
 
 Notation "x :: l" := (cons x l)
                      (at level 60, right associativity).
 Notation "[ ]" := nil.
 Notation "[ x ; .. ; y ]" := (cons x .. (cons y nil) ..).
 
-
-(* Definition xlist := [1;1;1;1]. *)
-
-(* Check ([1; 2; 3; 4]). *)
-
-(* Check (var1 [1; 2; 3]). *)
-
-
-
-  
-(* Inductive terms : Set := *)
-(* | var : string -> terms *)
-(* | app : string -> terms list -> terms. *)
-
 Inductive term : Set :=
-| var : nat -> term
-| fn  : nat -> term -> term.
+| var : nat -> term.
+(* | fn  : nat -> term -> term. *)
 
-Check fn 1 (fn 1 (var 2)).
+(* Check fn 1 (fn 1 (var 2)). *)
 
 Inductive form : Set :=
 | eq : term -> term -> form.
 
-Notation "x -=- y" := (eq x y)
-                        (at level 60).
-
-Check (fn 1 (var 2)) -=- (var 2).
-
-(* Check exists  *)
-
-(* Inductive prf (l : list (term * term)) : term -> Prop := *)
-(*   prfrefl (a : term) : (prf l a). *)
-
-
-(* Inductive prf (l : list (term * term)) (a : term) : term -> Prop := *)
-(*   prfrefl : prf l a a *)
-(*   prfsym  : prf l a b -> prf l b a.  *)
-
-
 (* The correctness condition *)
-
 Inductive prf (l : list (term * term)) : term -> term -> Prop  :=
-(* | paxm  :  *)  
-| pref : forall t, prf l t t
-| psym : forall s t, prf l s t -> prf l t s
-| ptrs : forall s t u, prf l s t -> prf l t u -> prf l s u
-| pcong : forall (n : nat) s t, prf l s t -> prf l (fn n s) (fn n t).
+  | paxm : forall s t, In (s, t) l -> prf l s t
+  | pref : forall t, prf l t t
+  | psym : forall s t, prf l s t -> prf l t s
+  | ptrs : forall s t u, prf l s t -> prf l t u -> prf l s u.
 
+
+Check paxm [(var 2, var 3)] (var 2) (var 3).
 
 Check psym [] (var 2) ( var 2) (pref [] (var 2) ).
 
-Check prf.  
-
-
+Check prf.
 
 (* computes all the subterms of a given term. *)
-
-Fixpoint subterms (t : term) : list term :=
+(* Fixpoint subterms (t : term) : list term :=
   match t with
   | var n => [var n]
   | fn n t1 => (fn n t1) :: subterms t1
+  end. *)
+Definition subterms (t:term) := 
+  match t with
+    | var n => [var n]
   end.
+
+Print Nat.eq_dec.
 
 (* give list of tuples of term and its parent *)
+Check beq_nat. (* Importes from EqNat *)
 
-Fixpoint parent_list (t : term) :=
-  match t with
-  | var _ => []
-  | fn n t => (t, fn n t) :: parent_list t
+(* Scheme Equality for term. (* screw these defs. *) *)
+(* Check term_beq. *)
+(* Check term_eq_dec. *)
+(* Print term_eq_dec. *)
+
+(* Define own term equality and nodup boolean version. *)
+(* Reset term_beq. (* Use IDE navigation?? *) *)
+Definition term_beq (a b : term) := 
+  match a, b with
+  | var n1, var n2 => beq_nat n1 n2
   end.
 
-Eval compute in parent_list (fn 1 (var 2)).
+Check term_beq.
+Compute term_beq (var 3) (var 4).
+Check nodup.
+Check in_dec.
 
-Scheme Equality for term.
-
-Check term_eq_dec.
-
-Eval compute in term_eq_dec (var 2) (fn 1 (var 3)).
-
-Eval compute in term_beq (var 2) (var 3).
-
-Eval compute in if (term_beq (var 2) (var 2)) then 1 else 0.
-
-
-(* Ignore this *)
-
-Definition f (t : term) (arg : term*term) :=
-  match arg with
-  | (x, _) => term_beq t x
+(* Define own nodup which works with (term->term->bool) *)
+Fixpoint skip {A:Type}  (f : A -> A -> bool) (e : A) (l : list A) : list A :=
+  match l with
+  | [] => []
+  | x::xs => if f e x then skip f e xs else x :: skip f e xs
   end.
-  
 
-(* gets the parents of a particular term from parent_list *)
+Compute length [].
+Lemma skip_nonincr : forall (A:Type) (f:A->A->bool) (e:A) (l:list A) , length (skip f e l) <= length l.
+Proof.
+  intros. induction l as [ | h l' IHl].
+  + reflexivity.
+  + simpl. case (f e h) eqn:val.
+    2:{
+      simpl. Search (_ <= _ -> S _ <= S _).
+      apply le_n_S, IHl. 
+      }
+    1:{
+      simpl. Print le. apply le_S. trivial.
+      }
+Qed.
+(* Program Fixpoint nodupb {A:Type} (f: A -> A -> bool) (l :list A) {wf show skip is nonincreasing} : list A :=
+  match l with
+  | [] => []
+  | x::xs => x :: nodupb f (skip f x xs)
+  end. *)
+Print In.
 
-Definition get_parents (t : term) (l : list (term*term)) :=
-  map (fun x => match x with | (_, n) => n end) (filter (f t) l).
+(* Fixpoint rem_el (f: A -> A -> bool) (a : A) (l : list A) := *)
 
-Eval compute in get_parents (var 2) (parent_list (fn 1 (var 2)) ++ parent_list (fn 3 (var 2))).
+Fixpoint check {A:Type} (f : A -> A -> bool) (x : A)  (acc : list A) :=
+  match acc with
+  | [] => false
+  | y::ys => if (f x y) then true else check f x ys
+  end.
+
+Fixpoint nodup_new {A:Type} (f: A -> A -> bool) (l : list A) (acc : list A) : list A :=
+ match l with
+ |  [] => acc
+ |  x::xs => if (check f x acc) then nodup_new f xs acc else nodup_new f xs (x::acc)
+ end.
 
 
-Check remove.
+Search "nodup".
 
-Check List.remove.
+Theorem nodup_nodup: forall (l tail: list term) (a x: term),
+    nodup_new (term_beq) l [] = a :: tail -> ~ In  a tail.
+Proof.
+  intros.
+  induction l.
+  + simpl in H. inversion H.
+  + simpl in H. 
+    
+                                                       
 
-Check last.
+(* Example check : term_eq_dec (var 3) (var 3). ??? *)
+(* Proof.
+Admitted. *)
 
-Eval compute in remove term_eq_dec (var 2) [var 2; var 3; var 4].
+(* Eval compute in term_eq_dec (var 2) (fn 1 (var 3)). *)
+(* Eval compute in term_beq (var 2) (var 3). *)
+(* Eval compute in if (term_beq (var 2) (var 2)) then 1 else 0. *)
 
-Definition removeT l := remove term_eq_dec (var 2) l.
-
+Notation "x -=- y" := (term_beq x y)
+                        (at level 60).
 
 (* Scheme Equality for term*term. *)
-
 Definition term_pairs_eqb (u v : term * term) :=
   match (u, v) with
   | ((a, b), (c, d)) => andb  (term_beq a c) (term_beq b d)
   end.
 
+Compute skip term_pairs_eqb (var 3, var 4) [(var 3, var 5); (var 3, var 4); (var 1, var 3)].
 
-(* equality for... *)
-(* Definition term_pairs_eq_dec (u v : term * term) := *)
-(*   match (u, v) with *)
-(*   | ((a, b), (c, d)) => (term_eq_dec a c) /\ (term_eq_dec b d) *)
-(*   end. *)
+(* Compute nodupb term_pairs_eqb [(var 3, var 5); (var 3, var 4); (var 1, var 3); (var 3, var 4)]. *)
 
-Definition removeTP a l := remove term_pairs_eq a l.
+Search "nodup".
 
-(* Setting up the UF datastructure. Will need further modification *)
+Fixpoint uf_find (l : list (term*term)) (t : term) :=
+  match l with
+  | [] => t (*  *)
+  | (x, y) :: ls => if term_beq x t then y
+                    else
+                      uf_find ls t
+  end.
 
-(* Fixpoint uf_find (l : list (term*term)) (t : term) := *)
+
+(* Fixpoint uf_find1 (l : list (term*term)) (t : term) := *)
 (*   match l with *)
-(*   | [] => var 1000 *)
-(*   | (x, y)::ls => if term_beq x t then (if term_beq x y then x else uf_find l y) else *)
-(*                     uf_find ls t *)
+(*   | [] => var (1000) *)
+(*   | (t, y) :: ls => y *)
+(*   | _ :: ls            =>  uf_find ls t *)
 (*   end. *)
 
 
-(* Fixpoint uf_merge (l : list (term*term)) (u v : term) := *)
-(*   let a := uf_find l u in *)
-(*   let b := uf_find l v in *)
-(*   if term_beq a b then l else remove *)
+Fixpoint change_rep (l : list (term * term)) (a b : term) :=
+  if term_beq a b then l else
+    match l with
+    | [] => []
+    | (x, n) :: xs => if term_beq n a then (x, b) :: change_rep xs a b
+                      else
+                        (x, n) :: change_rep xs a b
+    end.
 
 
-                    
-(* Ignore this *)
-(* Fixpoint get_parents (t : term) (l : list (term*nat)) := *)
-(*   match l with *)
-(*   | [] => [] *)
-(*   | (x,n) :: xs => match t with *)
-(*                    | x => n :: get_parents t xs *)
-(*                    | _ => get_parents t xs *)
-(*                    end *)
-                   
-(*   end. *)
+Definition uf_merge (l : list (term*term)) (u v : term) :=
+  let a := uf_find l u in
+  let b := uf_find l v in
+  change_rep l a b.
+
+
+Fixpoint do_cc (work ufl : list (term*term)) (bound : nat) :=
+  match bound with
+  | 0 => ufl
+  | _ => match work with
+         | [] => ufl
+         | (t1, t2) :: ws => ufl end
+  end.
+
+Fixpoint do_cc1 (work ufl : list (term*term)) :=
+  match work with
+  | [] => ufl
+  | (t1, t2) :: ws => do_cc1 ws (uf_merge ufl t1 t2)
+  end.
+
+Definition wfl' l ufl := forall c d, term_beq (uf_find ufl c) (uf_find ufl
+                                                                       d) =
+                                     true -> prf l c d.
+
+Theorem main_one' : forall l ufl, (wfl' l ufl) -> wfl' l (do_cc1 l ufl).
+Proof.
+  intros.
+  induction l.
+  simpl.
+  assumption.
+
+  destruct a.
+  simpl.
+
+  unfold wfl' in H, IHl. unfold wfl'. intros.
+  case (uf_find ufl c -=- uf_find ufl d) eqn: lets_try.
+  apply H in lets_try. assumption.
+  Admitted.
+
+  
+
+Definition wfl l ufl := forall c d, uf_find ufl c = d -> prf l c d.
+
+Theorem main_one : forall l ufl, (wfl l ufl) -> wfl l (do_cc1 l ufl).
+Proof.
+  intros.
+  (* unfold wfl. *)
+  (* unfold wfl in H. *)
+  (* intros. *)
+  (* inversion in H0. *)
+  (* inversion. *)
+  
+  (* induction l. *)
+  unfold wfl in *.
+  simpl.
+ Admitted.
+
+(*   (* unfold wfl. *) *)
+(*   (* unfold wfl in H, IHl. *) *)
+(*   destruct a. *)
+(*   simpl. *)
+(*   unfold wfl. unfold wfl in H, IHl. *)
+(*   intros. *)
+(*   pose (new1 := ((H t) (uf_find ufl t))). *)
+(*   assert (uf_find ufl t = uf_find ufl t). *)
+(*   reflexivity. *)
+(*   pose (shit := (new1 H1)). *)
+
+(*   pose (new2 := ((H t0) (uf_find ufl t0))). *)
+(*   assert (uf_find ufl t0 = uf_find ufl t0). *)
+(*   reflexivity. *)
+(*   pose (shit1 := (new2 H2)). *)
+
+  
+(*   (* unfold do_cc1 in H0. *) *)
+(*   (* case (uf_find ufl c) eqn: bagbose. *) *)
+(*   (* case (d) eqn: mad. *) *)
+(*   (* (* unfold wfl in H. *) *) *)
+(*   (* unfold wfl. *) *)
+(*   (* intros. *) *)
+(*   (* unfold wfl in IHl. *) *)
+(*   (* unfold uf_merge in H0. *) *)
+(*   (* case (uf_find ufl c = d) eqn: something. *) *)
+(*   (* unfold wfl. *) *)
+  
+(*   (* pose (nt := uf_find ufl t1). *) *)
+(*   (* Variable xy : uf_find ufl t1. *) *)
+(*   (* unfold change_rep. *) *)
+  
+(*   (* unfold uf_merge. *) *)
+(*   (* unfold do_cc1. *) *)
+(* admit.   *)
+
+Fixpoint create_uf' (l : list (term*term)) :=
+  match l with
+  | [] => [] 
+  | (t1, t2)::ls => (subterms t1 ++ subterms t2) ++ create_uf' ls
+  end.
+
+Print nodup_new.
+
+Definition create_uf l := let res := nodup_new term_beq (create_uf' l) []
+                          in map (fun x => (x, x)) res.
+
+Fixpoint cc1_algo (work : list (term*term)) (t1 t2 : term) : bool :=
+  (* let ufl := create_uf ((t1, t2)::work) in *)
+  let ufl := create_uf (work) in
+  let res := do_cc1 work ufl in
+  let a  := uf_find res t1 in
+  let b  := uf_find res t2 in
+  term_beq a b.
+
+Eval compute in cc1_algo [(var 1, var 2); (var 1, var 3); (var 3,var 4)] (var 2) (var 4).
+
+Eval compute in cc1_algo [(var 1, var 2); (var 1, var 3); (var 3,var 4); (var 5, var 6)] (var 3) (var 6).
+
+Search "nat_beq".
+Check nodup.
+
+Compute uf_find [(var 3, var 3)] (var 3).
+
+(* Theorem cc1_sound l a b: cc1_algo l a b = true -> prf l a b. *)
+(* Proof. *)
+(*   intros correct. induction l as [ | hl l' Hl]. *)
+(*   + simpl in correct. remember (create_uf [(a, b)]) as ufl. *)
+
+(*     unfold create_uf in Hequfl. simpl in Hequfl. rewrite app_nil_r in Hequfl. *)
+(*     destruct a as [ na ]; destruct b as [ nb ]. simpl subterms in Hequfl. *)
+(*     simpl app in Hequfl. simpl nodup_new in Hequfl. case (nb =? na) eqn:mast. *)
+(*     - simpl in Hequfl. Search (_=?_). *)
+(*       apply beq_nat_true in mast. rewrite mast. *)
+(*       apply pref. *)
+(*     - simpl in Hequfl. Search (_=?_).  *)
+(* (*     apply beq_nat_false in mast. Locate "<>". *) *)
+(*      rewrite Hequfl in correct. simpl in correct. *)
+(* (*      pose (T := beq_nat_false nb na mast). unfold not in T. *) *)
+(*      pose ( Q := Nat.eqb_sym na nb). *)
+(*      rewrite Q in correct. rewrite <- (beq_nat_refl nb) in correct.  *)
+(*      rewrite <- (beq_nat_refl na) in correct. rewrite mast in correct. *)
+(*      simpl term_beq in correct. rewrite Q in correct. rewrite mast in correct. *)
+(*      discriminate. *)
+(*       + case (cc1_algo l' a b) eqn: bose. *)
+(*         admit. *)
+        
+        
+        
+(* Admitted. *)
+
+
+Theorem term_beq_refl: forall a, term_beq a a  = true.
+Proof.
+  intros.
+  case (a) eqn: fuck.
+  unfold "-=-".
+  Locate "=?". Search eqb _ _.
+  simpl. apply Nat.eqb_refl.
+Qed.
+
+  
+Theorem uf_find_refl: forall l a,  uf_find l a -=- uf_find l a = true.
+Proof.
+  intros.
+  apply term_beq_refl.
+Qed.
+
+Theorem term_beq_sym: forall  a b,  term_beq a b = true ->
+                                    term_beq b a = true.
+Proof.
+  intros.
+  case a eqn: fuck.
+  case b eqn: fuck1.
+  simpl in H.
+  simpl. Search (eqb _ _ = eqb _ _).
+
+  rewrite Nat.eqb_sym. assumption.
+Qed.
+
+                
+
+Theorem uf_find_sym: forall l a b, uf_find l a -=- uf_find l b = true
+                                   ->  uf_find l b -=- uf_find l a = true.
+Proof.
+  intros.
+  case a eqn: fuck.
+  case b eqn: fuck1.
+  case l eqn: fuck2.
+  apply term_beq_sym. assumption.
+
+  apply term_beq_sym. assumption.
+Qed.
+
+Theorem term_beq_trans: forall a b c,  term_beq a b = true ->
+                                       term_beq b c = true ->
+                                       term_beq a c = true.
+Proof.
+  intros.
+  case a eqn: H1.
+  case b eqn: H2.
+  case c eqn: H3.
+  simpl in *. apply beq_nat_true in H. rewrite H.
+  assumption.
+ (* Search Nat.eqb. *)
+ (*
+ apply Nat.beq_nat_eq *)
+Qed.
+
+Theorem uf_find_trans: forall l a b c, uf_find l a -=- uf_find l b
+                                       = true ->
+                                       uf_find l b -=- uf_find l c
+                                       = true ->
+                                       uf_find l a -=- uf_find l c
+                                       = true.
+Proof.
+  intros.
+  case (a) eqn: fuck.
+  case (b) eqn: fuck1.
+  case (c) eqn: fuck2.
+  case (l) eqn: fuck3.
+  apply (term_beq_trans (var n) (var n0) (var n1)).
+  simpl in *. assumption.
+  simpl in *. assumption.
+  apply (term_beq_trans (uf_find (p :: l0) (var n))
+                        (uf_find (p :: l0) (var n0))
+                        (uf_find (p :: l0) (var n1))). assumption.
+  assumption.
+Qed.
+
+
+Theorem term_eqb_eq: forall a b, a -=- b = true ->
+                                 a = b.
+Proof.
+  intros.
+  case a eqn: fuck.
+  case b eqn: fuck1.
+  simpl in H. apply Nat.eqb_eq in H. rewrite H. reflexivity.
+Qed.
+  
+  
+Theorem uf_implies_in_list: forall l x a, uf_find l x -=- a = true
+                                          -> x -=- a = false                                                   -> In (x, a) l.
+Proof.
+  intros.
+  induction l.
+  - simpl in H. rewrite H in H0. discriminate.
+  - case a0 eqn: fuck.
+    simpl in H.
+    case (t -=- x) eqn: fuck1.
+    simpl. apply term_eqb_eq in fuck1. apply term_eqb_eq in H.
+    + rewrite fuck1, H in *. left. reflexivity.
+    + right. apply IHl. assumption.
+Qed.
+
+Theorem change_rep_eq: forall l x a b, In (x, a) l ->
+                                       uf_find l x -=- a = true ->
+                                       uf_find (change_rep l a b) x
+                                               -=-  b = true.
+Proof.
+  intros.
+  induction l. simpl in H. contradiction. simpl in H.
+  (*inversion H. admit.*) destruct H.
+  rewrite H. simpl. case (a -=- b) eqn: a_not_b.
+  simpl. rewrite (term_beq_refl x). assumption.
+  rewrite (term_beq_refl a). simpl. rewrite (term_beq_refl x).
+  apply term_beq_refl.
+
+  case a0 eqn: Anaught. simpl. case (a -=- b) eqn: ANB.
+  simpl. case (t -=- x) eqn: fuck. simpl in H0.
+  rewrite fuck in H0. apply (term_beq_trans t0 a b).
+  assumption. assumption.
+
+  simpl in H0. rewrite fuck in H0. apply (term_beq_trans (uf_find l x) a b). assumption. assumption.
+
+  case (t0 -=- a) eqn: fuck. case (t -=- x) eqn: fuck1.
+  simpl. rewrite fuck1. apply term_beq_refl.
+
+  simpl. rewrite fuck1. simpl in H0. rewrite fuck1 in H0.
+  apply (IHl H H0).
+
+  simpl. case (t -=- x) eqn: fuck1. simpl in H0. rewrite fuck1 in H0.
+  rewrite H0 in fuck. discriminate.
+
+  simpl in H0. rewrite fuck1 in H0. apply (IHl H H0).
+Qed.
+
+
+(* Theorem uf_merge_eq': forall l x y a b, In (x, a) l -> *)
+(*                                         In (y, a) l -> *)
+(*                                         uf_find l x -=- a = true -> *)
+(*                                         uf_find (uf_merge l a b) y *)
+(*                                                 -=- b = true. *)
+(* Proof. *)
+(*   intros. *)
+(*   induction l. *)
+(*   + simpl in H. contradiction. *)
+(*   + simpl in H, H0. *)
+(*     inversion H. *)
+(*     inversion H0. admit.  *)
+
+Definition ufl_wf (l : list (term*term)) := forall x y, In (x, y) l ->
+                                                        In (y, y) l.
+
+Definition ufl_wf' (l : list (term*term)) := forall x y, uf_find l x -=- y = true ->
+                                                        uf_find l y -=- y = true.
+
+Theorem in_monotonic : forall (l: list (term*term))
+                              (x: term) (a: term)
+                              (a0: term*term),
+    In (x, a) l -> In (x, a) (a0 :: l).
+Proof.
+  intros.
+  simpl.
+  right. assumption.
+Qed.
+
+
+Theorem uf_merge_eq': forall l x a b, ufl_wf' l ->
+                                      In (x, a) l ->
+                                      uf_find l x -=- a = true ->
+                                      uf_find (uf_merge l a b) x -=-
+                                            uf_find l b
+                                      = true.
+Proof.
+  intros.
+  induction l.
+  + simpl in H0. contradiction.
+  + simpl in H0. destruct H0. unfold uf_merge.
+  - rewrite H0. simpl. case (x -=- a) eqn: fuck.
+    case (x -=- b) eqn: fuck1. pose (fuck2 := term_beq_refl a).
+    rewrite fuck2. simpl. pose (fuck3 := term_beq_refl x).
+    rewrite fuck3. assumption.
+
+    case (a -=- uf_find l b) eqn: fuck2.
+    simpl. pose (fuck3 := term_beq_refl x). rewrite fuck3.
+    assumption.
+    *  pose (fuck3 := term_beq_refl a).
+       rewrite fuck3. simpl.
+
+
+    pose (fuck4 := term_beq_refl x). rewrite fuck4.
+    apply term_beq_refl.
+
+    * admit.
+    
+  - unfold uf_merge. apply change_rep_eq.
+    pose (fuck5 := (in_monotonic l x a a0 H0)).
+    unfold ufl_wf' in H. pose (fuck6 := (H x a H1)).
+    apply term_eqb_eq in fuck6. rewrite fuck6.
+    assumption.
+
+     unfold ufl_wf' in H. pose (fuck6 := (H x a H1)).
+     apply term_eqb_eq in fuck6. rewrite fuck6.
+     assumption.
+Admitted.     
 
 
 
+(* Theorem uf_merge_eq: forall l x a b, In (x, a) l -> *)
+(*                                      In (y, b) l -> *)
+(*                                      uf_find l x -=- a = true -> *)
+(*                                      uf_find (uf_merge l a b) x -=- *)
+(*                                              b *)
+(*                                      = true. *)
+(* Proof. *)
+(*   intros. *)
+(*   induction l. *)
+(*   + simpl in H. contradiction. *)
+(*   + simpl in H. destruct H. unfold uf_merge. *)
+(*   case l eqn: H1. *)
+(*   case x eqn: H2. *)
+(*   case a eqn: H3. *)
+(*   case b eqn: H4. *)
+(*   simpl in H. rewrite H in *. (*simpl.*) *)
+(*   - admit. *)
+(*   - admit. *)
+(*   - unfold uf_merge. *)
+(*     apply change_rep_eq with (l := (a0 :: l) *)
+(*                                    (x := x) *)
+(*                                    (a := (uf_find (a0 :: l) a)) *)
+(*                                    (b := (uf_find (a0 :: l) b))). *)
+
+(*     Abort. *)
+  (* unfold uf_merge. *)
+  (* simpl. simpl in H. apply beq_nat_true in H. *)
+  (* rewrite H. case (n0 =? n1) eqn: doit. admit. simpl in H. simpl. admit. Admitted. *)
+                                       
+
+Theorem cc1_mon: forall work x y a b, cc1_algo work a b = true ->
+                                      cc1_algo ((x, y) :: work) a b = true.
+Proof.
+  intros.
+  
+  induction work.
+  
+  {simpl. simpl in H. apply term_eqb_eq in H.
+   rewrite H. 
+   unfold cc1_algo. apply uf_find_refl. }
+
+  { destruct a0. simpl. case x eqn: fuck1.
+    case y eqn: fuck2. unfold create_uf. simpl.
+    case (n0 =? n) eqn: fuck3. simpl. admit. admit.}
+  
+  
+Admitted.
 
 
+Theorem cc1_head: forall work a b, cc1_algo ((a, b) :: work) a b = true.
+Proof.
+  intros.
+  simpl.
+  case (a) eqn: fuck1.
+  case (b) eqn: fuck2. simpl.
+  
+  
+  
+Admitted.
+
+Theorem do_cc1_mon: forall work l x y,
+    uf_find l x -=- uf_find l y = true ->
+    uf_find (do_cc1 work l) x -=-
+         uf_find (do_cc1 work l) y
+    = true.
+Proof.
+  intros.
+  induction work.
+  - simpl. assumption.
+
+  - destruct a. simpl. 
+Abort.
+
+Theorem do_cc1_inv: forall work l x y,
+    uf_find l x -=- uf_find l y = true ->
+    uf_find (do_cc1 work l) x -=- uf_find (do_cc1 work l) y = true.
+Proof.
+  intros.
+  induction work.
+  { simpl. assumption. }
+  { destruct a. simpl. induction l.
+    + simpl. destruct t, t0. unfold uf_merge.
+      simpl. case (n =? n0). assumption. assumption.
+
+    + 
+  simpl in H. admit.
+Abort.
+
+Theorem do_cc1_rewrite: forall work a l,
+    do_cc1 (a :: work) l = do_cc1 [a] (do_cc1 work l).
+Proof.
+  intros. destruct a.
+  induction l.
+  simpl. unfold uf_merge. simpl. case (t -=- t0).
+  
+
+Theorem do_cc1_mon_aux: forall work l x y
+  t t0,
+    uf_find (do_cc1 work l) x -=-
+            uf_find (do_cc1 work l) y
+    = true ->
+
+    uf_find (do_cc1 work (uf_merge l t t0))
+            x -=- uf_find (do_cc1 work (uf_merge l t t0)) y = true.
+Proof.
+  intros.
+  induction l as [ | a l'].
+  { unfold uf_merge. simpl.
+    case (t -=- t0). assumption.
+    assumption. }
+
+  { destruct a. unfold uf_merge. 
+    simpl.  unfold uf_merge. simpl.
+  
+                                                        
+                                  
+
+Theorem cc1_In: forall work a b, In (a, b) work ->
+                                 cc1_algo work a b = true.
+Proof.
+  intros.
+  (* unfold cc1_algo. *)
+  case (a) eqn: fuck.
+  case (b) eqn: fuck1.
+  induction work as [ | a0 work']. simpl in H. contradiction.
+  case (a0) eqn: fuck3.
+
+  simpl in H. destruct H.
+  { rewrite H. apply cc1_head. }
+  { apply cc1_mon. apply IHwork'. assumption. }  
+Qed.
 
 
+Theorem cc1_refl: forall work a, cc1_algo work a a = true.
+Proof.
+  intros.
+  case a eqn: fuck.
+  case work eqn: fuck2.
+  simpl.
+  apply Nat.eqb_refl.
+  (* apply uf_find_refl. *)
 
+  simpl. apply uf_find_refl.
+Qed.
+
+
+Theorem cc1_sym: forall work a b, cc1_algo work a b = true ->
+                                  cc1_algo work b a = true.
+Proof.
+  intros.
+  unfold cc1_algo in *.
+  case (a) eqn: fuck.
+  case (b) eqn: fuck1.
+  case (work) eqn: fuck2.
+  apply uf_find_sym. assumption.
+  apply uf_find_sym. assumption.
+Qed.
+
+
+Theorem cc1_trans: forall work a b c, cc1_algo work a b = true ->
+                                      cc1_algo work b c = true ->
+                                      cc1_algo work a c = true.
+Proof.
+  intros.
+  unfold cc1_algo in *.
+  case (a) eqn: fuck.
+  case (b) eqn: fuck1.
+  case (c) eqn: fuck2.
+  case (work) eqn: fuck3.
+  
+  apply (uf_find_trans
+           (do_cc1 [] (create_uf [])) (var n)
+           (var n0) (var n1)). assumption. assumption.
+
+
+  apply (uf_find_trans
+           (do_cc1 (p :: l) (create_uf (p :: l))) (var n)
+           (var n0) (var n1)).
+  assumption. assumption.
+Qed.
+
+
+Theorem cc1_complete work a b: prf work a b -> cc1_algo work a b = true.
+Proof.
+(*   intros proof. inversion proof. *)
+(*   + admit. (* In the list case*) *)
+(*   + admit. (* case of reflexivity *) *)
+(*   +  *)
+(*   + *)
+  (* Admitted. *)
+
+  intros. induction H.
+  + apply cc1_In. assumption. (* case: in the list *)
+  + apply cc1_refl. (* case: refl *)
+  + apply cc1_sym. assumption. (* case: sym of cc algo *)
+  + apply (cc1_trans work s t u). (* case: trans of cc algo *)
+    assumption.
+    assumption.
+Qed.
+
+Fixpoint create_uf' (l : list (term*term)) :=
+  match l with
+  | [] => [] 
+  | (t1, t2)::ls => (subterms t1 ++ subterms t2) ++ create_uf' ls
+  end.
+
+Check nodup_new.
+
+Definition create_uf l := let res := nodup_new term_eq_dec  (create_uf' l)
+                          in map (fun x => (x, x)) res.
+
+Check fold_left.
+
+Definition create_parents l :=
+  let lis := fold_left (fun x y => x ++ y) (map parent_list1 l) []
+  in map (fun x => (x, get_parents1 x lis)) l.
+                          
+
+Definition cc_algo (l : list (term*term)) (a b : term) :=
+  (* do the merging *)
+  let res := 1 in
+  let t1  := uf_find l a in
+  let t2  := uf_find l b in
+  term_beq t1 t2.
